merge proof reduced to diff_s proof

fqueue2.fst
@@ -401,9 +401,10 @@ assume val axiom_ae : l:ae
                            (forall e. mem e l.l ==> not (l.vis e e) (*irreflexive*) ))
                            [SMTPat (unique l.l)]
 
-val matched : e:o{is_enqueue e} -> d:o{is_dequeue d} -> tr:ae{mem e tr.l /\ mem d tr.l /\ get_id e <> get_id d}
-            -> Tot (b:bool{(return d = Some (get_id e, get_ele e) /\ (tr.vis e d)) <==> (b = true)})
-let matched e d tr = (return d = Some (get_id e, get_ele e)) && (tr.vis e d)
+val matched : e:o -> d:o -> tr:ae
+            -> Pure bool (requires (get_id e <> get_id d))
+                        (ensures (fun b -> (is_enqueue e /\ is_dequeue d /\ mem e tr.l /\ mem d tr.l /\ return d = Some (get_id e, get_ele e) /\ (tr.vis e d)) <==> (b = true)))
+let matched e d tr = (is_enqueue e && is_dequeue d && mem e tr.l && mem d tr.l && return d = Some (get_id e, get_ele e)) && (tr.vis e d)
 
 val sub_list : e:o -> l:list o{mem e l /\ unique l} -> l1:list o{not (mem e l1) /\ unique l1 /\ (forall e. mem e l1 ==> mem e l) /\ length l1 <= length l}
 let rec sub_list e l = match l with
@@ -555,7 +556,7 @@ val sim0 : tr:ae
 let sim0 tr s0 =
     axiom_ae tr;
     let enq_list = filter_op (fun x -> is_enqueue x && mem x tr.l && not
-                             (exists_mem tr.l (fun d -> is_dequeue d && mem d tr.l && mem x tr.l && get_id x <> get_id d && matched x d tr))) tr.l in
+                             (exists_mem tr.l (fun d -> is_dequeue d && get_id x <> get_id d && matched x d tr))) tr.l in
     if forall_mem enq_list (fun x -> mem x tr.l && is_enqueue x && mem ((get_id x), (get_ele x)) (tolist s0)) &&
        forall_mem (tolist s0) (fun x -> mem ((fst x), Enqueue (snd x)) enq_list)
                             then true else false
@@ -707,12 +708,27 @@ let absmerge l a b =
                  (mem o l.l && mem o1 a.l && get_id o <> get_id o1 && (union l a).vis o o1) ||
                  (mem o l.l && mem o1 b.l && get_id o <> get_id o1 && (union l b).vis o o1)) (absmerge_list_ae l a b))
 
+
+val d0 : a: list(nat * nat)
+       -> x:(nat * nat)
+       -> Lemma (requires (unique_id a))
+               (ensures (not (mem_id (fst x) a) ==> not (mem (x) a)))
+let d0 a x = ()
+
 val diff_s : a:list (nat * nat)
            -> l:list (nat * nat)
            -> Pure (list (nat * nat))
-             (requires (unique_id a /\ unique_id l))
-             (ensures (fun d -> (forall e. mem e d <==> (mem e a /\ not (mem e l))) /\ unique_id d ))
-let diff_s a l = filter_s (fun e -> not (mem e l)) a
+             (requires (unique_id a /\ unique_id l /\ (forall e e1. mem e a /\ mem e1 l /\ (fst e = fst e1) ==> (snd e = snd e))))
+             (ensures (fun d -> (forall e. mem e d <==> (mem e a /\ not (mem e l))) /\ unique_id d /\ (forall e. mem_id e d <==> (mem_id e a /\ not (mem_id e l)))))
+
+let rec diff_s a l =  match a with
+  | [] -> []
+  | x::xs -> let d = (if (mem (x) l) then diff_s xs l else x::(diff_s xs l)) in
+           assert(forall e. mem_id e a /\ not (mem_id e l) ==> mem_id e d);
+           // assert(forall e. mem_id e d ==> (mem_id e a /\ not (mem_id e l)));
+           assert(forall e. mem e d ==> (mem e a /\ not (mem e l)));
+           assert(forall e. (mem e a /\ not (mem e l)) ==> mem e d); admit();
+           d
 
 val filter1 : f:((nat * nat) -> bool)
                -> l:list (nat * nat)
@@ -743,8 +759,7 @@ let intersection l a b =
 val union_s : a:list (nat * nat)
             -> b:list (nat * nat)
             -> Pure (list (nat * nat))
-              (requires unique_id a /\ unique_id b /\ (forall e. mem e a ==> not (mem_id (fst e) b)) /\ (forall e. mem e b ==> not (mem_id (fst e) a)) /\
-                                  (forall e e1. mem e a /\ mem e1 b ==> get_id e < get_id e1))
+              (requires unique_id a /\ unique_id b /\ (forall e. mem e a ==> not (mem_id (fst e) b)) /\ (forall e. mem e b ==> not (mem_id (fst e) a)))
               (ensures (fun u -> (forall e. mem e u <==> mem e a \/ mem e b) /\ unique_id u /\
                               (forall e e1. ((mem e a /\ mem e1 a /\ fst e <> fst e1 /\ order e e1 a) \/ (mem e b /\ mem e1 b /\ fst e <> fst e1 /\ order e e1 b) \/
                                              (mem e a /\ mem e1 b /\ fst e <> fst e1)) <==> (mem e u /\ mem e1 u /\ order e e1 u))))
@@ -839,28 +854,23 @@ val merge_s : l:list (nat * nat)
             -> Pure (list (nat * nat))
                    (requires unique_id a /\ unique_id l /\ unique_id b /\
                              (forall e. mem e (diff_s a l) ==> not (mem_id (fst e) (diff_s b l))) /\
-                             (forall e. mem e (diff_s b l) ==> not (mem_id (fst e) (diff_s a l))) // /\
-                             // (forall e e1. mem e l /\ mem e1 l /\ mem e a /\ mem e1 a /\ order e e1 l ==> order e e1 a) /\
-                             // (forall e e1. mem e l /\ mem e1 l /\ mem e b /\ mem e1 b /\ order e e1 l ==> order e e1 b)
-    )
+                             (forall e. mem e (diff_s b l) ==> not (mem_id (fst e) (diff_s a l))))
                    (ensures (fun res -> unique_id res /\ (forall e. mem e res <==> ((mem e l /\ mem e a /\ mem e b) \/
                                     (mem e a /\ not (mem e l)) \/ (mem e b /\ not (mem e l)))) /\
                                     (forall e. mem e l /\ not (mem e a) ==> not (mem e res)) /\
                                     (forall e. mem e l /\ not (mem e b) ==> not (mem e res)) /\
-                                    (forall e e1. mem e l /\ mem e1 l /\ fst e <> fst e1 /\ order e e1 l /\ mem e res /\ mem e1 res ==> order e e1 res) /\
-                                    (forall e e1. mem e a /\ mem e1 a /\ fst e <> fst e1 /\ order e e1 a /\ mem e res /\ mem e1 res ==> order e e1 res) /\
-                                    (forall e e1. mem e b /\ mem e1 b /\ fst e <> fst e1 /\ order e e1 b /\ mem e res /\ mem e1 res ==> order e e1 res) /\
-                                    (forall e e1. mem e l /\ mem e1 (diff_s a l) /\ fst e <> fst e1 /\ mem e res /\ mem e1 res ==> order e e1 res) /\
-                                    (forall e e1. mem e l /\ mem e1 (diff_s b l) /\ fst e <> fst e1 /\ mem e res /\ mem e1 res ==> order e e1 res) /\
-                                    (forall e e1. (mem e (diff_s a l) /\ mem e1 (diff_s b l) /\ (fst e < fst e1))
-                                         ==> order e e1 res)))
+                                    (forall e e1. ((mem e l /\ mem e1 l /\ fst e <> fst e1 /\ order e e1 l /\ mem e res /\ mem e1 res) \/
+                                      (mem e l /\ mem e1 (diff_s a l) /\ fst e <> fst e1 /\ mem e res /\ mem e1 res) \/
+                                      (mem e l /\ mem e1 (diff_s b l) /\ fst e <> fst e1 /\ mem e res /\ mem e1 res) \/
+                                      (mem e (diff_s a l) /\ mem e1 (diff_s b l) /\ (fst e < fst e1))) ==>
+                                       (mem e res /\ mem e1 res /\ fst e <> fst e1 /\ order e e1 res))))
 
 let merge_s l a b =
   let ixn = intersection l a b in
   let diff_a = diff_s a l in
   let diff_b = diff_s b l in
   let union_ab = sorted_union diff_a diff_b in
-  admit(); union_s ixn union_ab
+    union_s ixn union_ab
 
 val merge : ltr:ae
           -> l:s
@@ -880,19 +890,91 @@ val merge : ltr:ae
                                 (memq e a /\ not (memq e l)) \/ (memq e b /\ not (memq e l)))) /\
                                 (forall e. memq e l /\ not (memq e a) ==> not (memq e res)) /\
                                 (forall e. memq e l /\ not (memq e b) ==> not (memq e res)) /\
-                                (forall e e1. memq e l /\ memq e1 l /\ fst e <> fst e1 /\ order e e1 (tolist l) /\ memq e res /\ memq e1 res ==> order e e1 (tolist res)) /\
-                                (forall e e1. memq e a /\ memq e1 a /\ fst e <> fst e1 /\ order e e1 (tolist a) /\ memq e res /\ memq e1 res ==> order e e1 (tolist res)) /\
-                                (forall e e1. memq e b /\ memq e1 b /\ fst e <> fst e1 /\ order e e1 (tolist b) /\ memq e res /\ memq e1 res ==> order e e1 (tolist res)) /\
-                                (forall e e1. memq e l /\ mem e1 (diff_s (tolist a) (tolist l)) /\ fst e <> fst e1 /\ memq e res /\ memq e1 res ==> order e e1 (tolist res)) /\
-                                (forall e e1. memq e l /\ mem e1 (diff_s (tolist b) (tolist l)) /\ fst e <> fst e1 /\ memq e res /\ memq e1 res ==> order e e1 (tolist res)) /\
-                           (forall e e1. (mem e (diff_s (tolist a) (tolist l)) /\ mem e1 (diff_s (tolist b) (tolist l)) /\ (fst e < fst e1)) ==> order e e1 (tolist res))
+                                (forall e e1. ((memq e l /\ memq e1 l /\ fst e <> fst e1 /\ order e e1 (tolist l) /\ memq e res /\ memq e1 res) \/
+                                      (memq e l /\ mem e1 (diff_s (tolist a) (tolist l)) /\ fst e <> fst e1 /\ memq e res /\ memq e1 res) \/
+                                      (memq e l /\ mem e1 (diff_s (tolist b) (tolist l)) /\ fst e <> fst e1 /\ memq e res /\ memq e1 res) \/
+                                      (mem e (diff_s (tolist a) (tolist l)) /\ mem e1 (diff_s (tolist b) (tolist l)) /\ (fst e < fst e1))) <==>
+                                       (memq e res /\ memq e1 res /\ fst e <> fst e1 /\ order e e1 (tolist res)))
                             ))
 
-#push-options "--initial_fuel 4 --ifuel 4 --initial_ifuel 4 --fuel 4 --z3rlimit 1000"
+#push-options "--initial_fuel 6 --ifuel 6 --initial_ifuel 6 --fuel 6 --z3rlimit 10000"
 
 let merge ltr l atr a btr b = (S (merge_s (tolist l) (tolist a) (tolist b)) [])
 
-#pop-options
+val prop_merge0 : ltr: ae
+                -> l:s
+                -> atr:ae
+                -> a:s
+                -> btr:ae
+                -> b:s
+                -> Lemma (requires ((forall e. mem e ltr.l ==> not (member (get_id e) atr.l)) /\
+                                   (forall e. mem e ltr.l ==> not (member (get_id e) btr.l)) /\
+                                   (forall e. mem e atr.l ==> not (member (get_id e) btr.l)) /\
+                                   (forall e e1. (mem e ltr.l /\ mem e1 atr.l ==> get_id e < get_id e1)) /\
+                                   (forall e e1. (mem e ltr.l /\ mem e1 btr.l ==> get_id e < get_id e1)) /\
+                                   (sim ltr l /\ sim (union ltr atr) a /\ sim (union ltr btr) b) /\
+                                   (forall e. mem_id e (diff_s (tolist a) (tolist l)) ==> not (mem_id e (diff_s (tolist b) (tolist l)))) /\
+                                   (forall e. mem_id e (diff_s (tolist b) (tolist l)) ==> not (mem_id e (diff_s (tolist a) (tolist l))))))
+                       (ensures (sim0 (absmerge ltr atr btr) (merge ltr l atr a btr b)))
+
+let prop_merge0 ltr l atr a btr b =
+  axiom_ae ltr; axiom_ae atr; axiom_ae btr; axiom_ae (union ltr atr); axiom_ae (union ltr btr);
+  let tr = absmerge ltr atr btr in
+  let s0 = merge ltr l atr a btr b in
+  let enq_list = filter_op (fun x -> is_enqueue x && mem x tr.l && not
+                             (exists_mem tr.l (fun d -> is_dequeue d && mem d tr.l && mem x tr.l && get_id x <> get_id d && matched x d tr))) tr.l in
+
+  let enq_list1 = filter_op (fun x -> is_enqueue x && mem x ltr.l && not
+                             (exists_mem ltr.l (fun d -> is_dequeue d && mem d ltr.l && mem x ltr.l && get_id x <> get_id d && matched x d ltr))) ltr.l in
+
+  let enq_list2 = filter_op (fun x -> is_enqueue x && mem x (union ltr atr).l && not
+                             (exists_mem (union ltr atr).l (fun d -> is_dequeue d && mem d (union ltr atr).l && mem x (union ltr atr).l &&
+                                         get_id x <> get_id d && matched x d (union ltr atr)))) (union ltr atr).l in
+
+  let enq_list3 = filter_op (fun x -> is_enqueue x && mem x (union ltr btr).l && not
+                             (exists_mem (union ltr btr).l (fun d -> is_dequeue d && mem d (union ltr btr).l && mem x (union ltr btr).l &&
+                                         get_id x <> get_id d && matched x d (union ltr btr)))) (union ltr btr).l in
+
+  let enq_list4 = filter_op (fun x -> is_enqueue x && mem x atr.l && not
+                             (exists_mem atr.l (fun d -> is_dequeue d && mem d atr.l && mem x atr.l && get_id x <> get_id d && matched x d atr))) atr.l in
+
+  let enq_list5 = filter_op (fun x -> is_enqueue x && mem x btr.l && not
+                             (exists_mem btr.l (fun d -> is_dequeue d && mem d btr.l && mem x btr.l && get_id x <> get_id d && matched x d btr))) btr.l in
+
+  // VVGG assert(forall e. (mem e enq_list2 /\ mem e enq_list3) \/ ((mem e enq_list4) \/ (mem e enq_list5)) ==> mem e enq_list);
+  // VVGG assert(forall e. (mem e enq_list2 /\ mem e enq_list3) \/ ((mem e enq_list4) \/ (mem e enq_list5)) ==> memq (get_id e, get_ele e) s0);
+  // VVGG assert(forall e. mem e enq_list4 ==> mem e enq_list2);
+  // VVGG assert(forall e. mem e enq_list5 ==> mem e enq_list3);
+  // VVGG assert(forall e. mem e enq_list2 /\ mem e enq_list3 <==> memq (get_id e, get_ele e) a /\ memq (get_id e, get_ele e) b /\ memq (get_id e, get_ele e) l);
+  // VVGG assert(forall e. mem e enq_list4 ==> (memq (get_id e, get_ele e) a /\ not(memq (get_id e, get_ele e) l)));
+  // VVGG assert(forall e. mem e enq_list5 ==> memq (get_id e, get_ele e) b /\ not(memq (get_id e, get_ele e) l));
+  // GG assert(forall e. mem e tr.l ==> (mem e (union ltr atr).l /\ mem e (union ltr btr).l) \/ mem e atr.l \/ mem e btr.l);
+  // assert(forall x. ((exists_mem tr.l (fun d -> is_dequeue d && get_id x <> get_id d && matched x d tr))) ==>
+
+  //          (((exists_mem (union ltr atr).l (fun d -> is_dequeue d && get_id x <> get_id d && matched x d (union ltr atr))) /\
+  //          ((exists_mem (union ltr btr).l (fun d -> is_dequeue d && get_id x <> get_id d && matched x d (union ltr btr))))) \/
+
+  //          ((exists_mem atr.l (fun d -> is_dequeue d && get_id x <> get_id d && matched x d atr))) \/
+  //          ((exists_mem btr.l (fun d -> is_dequeue d && get_id x <> get_id d && matched x d btr)))
+  //          ));
+
+  // assert(forall e d. is_enqueue e /\ is_dequeue d /\ mem e atr.l /\ mem d atr.l /\ get_id e <> get_id d /\ matched e d atr ==> matched e d tr);
+
+  // assert(forall f. exists_mem tr.l f ==> (exists_mem (union ltr atr).l f /\ exists_mem (union ltr btr).l f) \/ exists_mem atr.l f \/ exists_mem btr.l f);
+
+  // assert(forall e. mem e enq_list ==> ((mem e enq_list2 /\ mem e enq_list3) \/ ((mem e enq_list4) \/ (mem e enq_list5))));
+  // assert(forall e. mem e enq_list ==> memq (get_id e, get_ele e) s0);
+
+
+  // VVGG assert(forall e. ((memq e a /\ memq e b /\ memq e l) \/ (mem e (diff_s (tolist a) (tolist l))) \/ (mem e (diff_s (tolist b) (tolist l)))) ==>
+  //          mem (fst e, Enqueue (snd e)) enq_list);
+  // VVGG assert(forall e. ((memq e a /\ memq e b /\ memq e l) \/ (mem e (diff_s (tolist a) (tolist l))) \/ (mem e (diff_s (tolist b) (tolist l)))) <==>
+  //          memq e s0);
+  // VVGG assert(forall e. memq e s0 ==> mem (fst e, Enqueue (snd e)) enq_list);
+  // VVGG assert(forall_mem (tolist s0) (fun e -> mem (fst e, Enqueue (snd e)) enq_list));
+  admit();
+  ()
+
 
 val convergence : tr:ae
                 -> a:s
@@ -980,68 +1062,8 @@ let prop_oper tr st op =
   prop_oper6 tr st op;
   ()
 
-val prop_merge0 : ltr: ae
-                -> l:s
-                -> atr:ae
-                -> a:s
-                -> btr:ae
-                -> b:s
-                -> Lemma (requires ((forall e. mem e ltr.l ==> not (member (get_id e) atr.l)) /\
-                                   (forall e. mem e ltr.l ==> not (member (get_id e) btr.l)) /\
-                                   (forall e. mem e atr.l ==> not (member (get_id e) btr.l)) /\
-                                   (forall e e1. (mem e ltr.l /\ mem e1 atr.l ==> get_id e < get_id e1)) /\
-                                   (forall e e1. (mem e ltr.l /\ mem e1 btr.l ==> get_id e < get_id e1)) /\
-                                   (sim ltr l /\ sim (union ltr atr) a /\ sim (union ltr btr) b) /\
-                                   (forall e. mem_id e (diff_s (tolist a) (tolist l)) ==> not (mem_id e (diff_s (tolist b) (tolist l))))/\
-                                   (forall e. mem_id e (diff_s (tolist b) (tolist l)) ==> not (mem_id e (diff_s (tolist a) (tolist l))))))
-                       (ensures (sim0 (absmerge ltr atr btr) (merge ltr l atr a btr b)))
-
-let prop_merge0 ltr l atr a btr b =
-  axiom_ae ltr; axiom_ae atr; axiom_ae btr; axiom_ae (union ltr atr); axiom_ae (union ltr btr);
-  let tr = absmerge ltr atr btr in
-  let s0 = merge ltr l atr a btr b in
-  let enq_list = filter_op (fun x -> is_enqueue x && mem x tr.l && not
-                             (exists_mem tr.l (fun d -> is_dequeue d && mem d tr.l && mem x tr.l && get_id x <> get_id d && matched x d tr))) tr.l in
-
-  let enq_list1 = filter_op (fun x -> is_enqueue x && mem x ltr.l && not
-                             (exists_mem ltr.l (fun d -> is_dequeue d && mem d ltr.l && mem x ltr.l && get_id x <> get_id d && matched x d ltr))) ltr.l in
-
-  let enq_list2 = filter_op (fun x -> is_enqueue x && mem x (union ltr atr).l && not
-                             (exists_mem (union ltr atr).l (fun d -> is_dequeue d && mem d (union ltr atr).l && mem x (union ltr atr).l &&
-                                         get_id x <> get_id d && matched x d (union ltr atr)))) (union ltr atr).l in
-
-  let enq_list3 = filter_op (fun x -> is_enqueue x && mem x (union ltr btr).l && not
-                             (exists_mem (union ltr btr).l (fun d -> is_dequeue d && mem d (union ltr btr).l && mem x (union ltr btr).l &&
-                                         get_id x <> get_id d && matched x d (union ltr btr)))) (union ltr btr).l in
-
-  let enq_list4 = filter_op (fun x -> is_enqueue x && mem x atr.l && not
-                             (exists_mem atr.l (fun d -> is_dequeue d && mem d atr.l && mem x atr.l && get_id x <> get_id d && matched x d atr))) atr.l in
-
-  let enq_list5 = filter_op (fun x -> is_enqueue x && mem x btr.l && not
-                             (exists_mem btr.l (fun d -> is_dequeue d && mem d btr.l && mem x btr.l && get_id x <> get_id d && matched x d btr))) btr.l in
-
-  // VVGG
-  assert(forall e. (mem e enq_list2 /\ mem e enq_list3) \/ ((mem e enq_list4) \/ (mem e enq_list5)) ==> mem e enq_list);
-  // VVGG assert(forall e. (mem e enq_list2 /\ mem e enq_list3) \/ ((mem e enq_list4) \/ (mem e enq_list5)) ==> memq (get_id e, get_ele e) s0);
-  // VVGG assert(forall e. ((mem e enq_list4) \/ (mem e enq_list5)) ==> mem e enq_list);
-  // VVGG assert(forall e. mem e enq_list4 ==> mem e enq_list2);
-  // VVGG assert(forall e. mem e enq_list5 ==> mem e enq_list3);
-  // GG assert(forall e. mem e enq_list2 ==> (mem e (absmerge ltr atr btr).l));
-  // GG assert(forall e1. mem e1 (union ltr btr).l ==> (mem e1 (absmerge ltr atr btr).l));
-  // assert(forall e e1. mem e enq_list2 /\ mem e1 (union ltr btr).l /\ is_dequeue e1 /\ not(matched e e1 (absmerge ltr atr btr)) ==> mem e enq_list);
-  // assert(forall e e1. mem e enq_list2 /\ mem e1 (union ltr btr).l /\ is_dequeue e1 /\ not(matched e e1 (absmerge ltr atr btr)) ==> memq (get_id e, get_ele e) s0);
-  // assert(forall e. mem e enq_list ==> memq (get_id e, get_ele e) s0);
-  // VVGG assert(forall e. ((memq e a /\ memq e b /\ memq e l) \/ (mem e (diff_s (tolist a) (tolist l))) \/ (mem e (diff_s (tolist b) (tolist l)))) ==>
-  //          mem (fst e, Enqueue (snd e)) enq_list);
-  // VVGG assert(forall e. ((memq e a /\ memq e b /\ memq e l) \/ (mem e (diff_s (tolist a) (tolist l))) \/ (mem e (diff_s (tolist b) (tolist l)))) <==>
-  //          memq e s0);
-  // VVGG assert(forall e. memq e s0 ==> mem (fst e, Enqueue (snd e)) enq_list);
-  // VVGG assert(forall_mem (tolist s0) (fun e -> mem (fst e, Enqueue (snd e)) enq_list));
-  admit();
-  ()
-
-
 #set-options "--initial_fuel 10 --ifuel 10 --initial_ifuel 10 --fuel 10 --z3rlimit 1000000"
+
 
 val prop_merge1 : ltr: ae
                 -> l:s
